Simplify the proof about MlKemMod

proofs/Symcrust/Properties.lean
@@ -13,7 +13,6 @@ open Result
 
 namespace Aeneas.Std
 
-@[reducible]
 def ScalarTy.bitWidth (ty : ScalarTy) : Nat :=
   match ty with
   | Isize | Usize => size_num_bits
@@ -22,6 +21,19 @@ def ScalarTy.bitWidth (ty : ScalarTy) : Nat :=
   | I32 | U32 => 32
   | I64 | U64 => 64
   | I128 | U128 => 128
+
+@[simp] theorem ScalarTy.Isize_bitWidth : Isize.bitWidth = size_num_bits := by rfl
+@[simp] theorem ScalarTy.I8_bitWidth : I8.bitWidth = 8 := by rfl
+@[simp] theorem ScalarTy.I16_bitWidth : I16.bitWidth = 16 := by rfl
+@[simp] theorem ScalarTy.I32_bitWidth : I32.bitWidth = 32 := by rfl
+@[simp] theorem ScalarTy.I64_bitWidth : I64.bitWidth = 64 := by rfl
+@[simp] theorem ScalarTy.I128_bitWidth : I128.bitWidth = 128 := by rfl
+@[simp] theorem ScalarTy.Usize_bitWidth : Usize.bitWidth = size_num_bits := by rfl
+@[simp] theorem ScalarTy.U8_bitWidth : U8.bitWidth = 8 := by rfl
+@[simp] theorem ScalarTy.U16_bitWidth : U16.bitWidth = 16 := by rfl
+@[simp] theorem ScalarTy.U32_bitWidth : U32.bitWidth = 32 := by rfl
+@[simp] theorem ScalarTy.U64_bitWidth : U64.bitWidth = 64 := by rfl
+@[simp] theorem ScalarTy.U128_bitWidth : U128.bitWidth = 128 := by rfl
 
 theorem ScalarTy.unsigned_min_eq_zero (ty : ScalarTy) (h : ¬ty.isSigned) :
   Scalar.min ty = 0 := by
@@ -37,23 +49,41 @@ set_option maxRecDepth 1000
 open Result
 
 /-- Bit vector representation of a scalar -/
-def Scalar.bv {ty} (x : Scalar ty) : BitVec ty.bitWidth :=
+def Scalar.bv_ {ty} (x : Scalar ty) : BitVec ty.bitWidth :=
   if ty.isSigned then BitVec.ofInt _ x.val else BitVec.ofNat _ x.toNat
 
+def U8.bv (x : U8) : BitVec 8 := Scalar.bv_ x
+def U16.bv (x : U16) : BitVec 16 := Scalar.bv_ x
+def U32.bv (x : U32) : BitVec 32 := Scalar.bv_ x
+def U64.bv (x : U64) : BitVec 64 := Scalar.bv_ x
+def U128.bv (x : U128) : BitVec 128 := Scalar.bv_ x
+def Usize.bv (x : Usize) : BitVec size_num_bits := Scalar.bv_ x
+def I8.bv (x : I8) : BitVec 8 := Scalar.bv_ x
+def I16.bv (x : I16) : BitVec 16 := Scalar.bv_ x
+def I32.bv (x : I32) : BitVec 32 := Scalar.bv_ x
+def I64.bv (x : I64) : BitVec 64 := Scalar.bv_ x
+def I128.bv (x : I128) : BitVec 128 := Scalar.bv_ x
+def Isize.bv (x : Isize) : BitVec size_num_bits := Scalar.bv_ x
 
 @[simp]
 theorem Scalar.bv_toNat_eq {ty : ScalarTy} (x : Scalar ty) (h : ¬ ty.isSigned := by simp) :
-  (Scalar.bv x).toNat  = x.val := by
+  (Scalar.bv_ x).toNat  = x.toNat := by
   have := x.hmin
   have := x.hmax
-  simp [Scalar.bv, h]
+  simp [Scalar.bv_, h]
   simp [ScalarTy.unsigned_max_eq_pow_bitWidth, ScalarTy.unsigned_min_eq_zero, h] at *
-  simp [*]
-  have : x.val < 2 ^ ty.bitWidth := by omega
-  apply Int.emod_eq_of_lt <;> omega
+  have h := (System.Platform.getNumBits ()).property
+  dcases ty <;> simp_all <;> (try omega) <;>
+  dcases h <;> simp_all <;> omega
+
+@[simp] theorem U8.bv_toNat_eq (x : U8) : x.bv.toNat = x.toNat := by apply Scalar.bv_toNat_eq; simp
+@[simp] theorem U16.bv_toNat_eq (x : U16) : x.bv.toNat = x.toNat := by apply Scalar.bv_toNat_eq; simp
+@[simp] theorem U32.bv_toNat_eq (x : U32) : x.bv.toNat = x.toNat := by apply Scalar.bv_toNat_eq; simp
+@[simp] theorem U64.bv_toNat_eq (x : U64) : x.bv.toNat = x.toNat := by apply Scalar.bv_toNat_eq; simp
+@[simp] theorem U128.bv_toNat_eq (x : U128) : x.bv.toNat = x.toNat := by apply Scalar.bv_toNat_eq; simp
 
 theorem core.num.Scalar.wrapping_add_bv_unsigned_eq {ty} (x y : Scalar ty) (hs : ¬ ty.isSigned := by simp) :
-  (Scalar.wrapping_add x y).bv = x.bv + y.bv := by
+  (Scalar.wrapping_add x y).bv_ = x.bv_ + y.bv_ := by
   sorry
 
 theorem core.num.Scalar.wrapping_add_val_unsigned_eq {ty} (x y : Scalar ty) (hs : ¬ ty.isSigned := by simp) :
@@ -124,6 +154,26 @@ theorem core.num.Scalar.wrapping_add_toNat_unsigned_eq {ty} (x y : Scalar ty) (h
   (core.num.U128.wrapping_add x y).toNat = (x.toNat + y.toNat) % (U128.max + 1) :=
   core.num.Scalar.wrapping_add_toNat_unsigned_eq x y
 
+theorem core.num.Scalar.wrapping_sub_bv_unsigned_eq {ty} (x y : Scalar ty) (hs : ¬ ty.isSigned := by simp) :
+  (Scalar.wrapping_sub x y).bv_ = x.bv_ - y.bv_ := by
+  sorry
+
+@[simp] theorem core.num.U8.wrapping_sub_bv_eq (x y : U8) :
+  (core.num.U8.wrapping_sub x y).bv = x.bv - y.bv :=
+  core.num.Scalar.wrapping_sub_bv_unsigned_eq x y
+
+@[simp] theorem core.num.U16.wrapping_sub_bv_eq (x y : U16) :
+  (core.num.U16.wrapping_sub x y).bv = x.bv - y.bv :=
+  core.num.Scalar.wrapping_sub_bv_unsigned_eq x y
+
+@[simp] theorem core.num.U32.wrapping_sub_bv_eq (x y : U32) :
+  (core.num.U32.wrapping_sub x y).bv = x.bv - y.bv :=
+  core.num.Scalar.wrapping_sub_bv_unsigned_eq x y
+
+@[simp] theorem core.num.U64.wrapping_sub_bv_eq (x y : U64) :
+  (core.num.U64.wrapping_sub x y).bv = x.bv - y.bv :=
+  core.num.Scalar.wrapping_sub_bv_unsigned_eq x y
+
 theorem core.num.Scalar.wrapping_sub_val_unsigned_eq {ty} (x y : Scalar ty) (hs : ¬ ty.isSigned := by simp) :
   (Scalar.wrapping_sub x y).val = (x.val - y.val) % 2^ty.bitWidth := by
   sorry
@@ -177,19 +227,78 @@ theorem core.num.Scalar.wrapping_sub_toNat_unsigned_eq {ty} (x y : Scalar ty) (h
   (n % m).toNat = n % m := by
   simp only [Int.ofNat_toNat, ne_eq, h, not_false_eq_true, Int.emod_nonneg, sup_of_le_left]
 
-@[pspec] theorem core.num.Scalar.ShiftRight_val_unsigned_eq {ty0 ty1} (x : Scalar ty0) (y : Scalar ty1)
+theorem core.num.Scalar.ShiftRight_val_unsigned_eq {ty0 ty1} (x : Scalar ty0) (y : Scalar ty1)
   (hs : ¬ ty0.isSigned) (hy0 : 0 ≤ y.val) (hy1 : y.val ≤ ty0.bitWidth) :
   ∃ z, x >>> y = ok z ∧
   z.val = x.val >>> y.toNat
   := by
   sorry
 
-@[pspec] theorem core.num.Scalar.ShiftLeft_val_unsigned_eq {ty0 ty1} (x : Scalar ty0) (y : Scalar ty1)
+theorem core.num.Scalar.ShiftRight_bv_unsigned_eq {ty0 ty1} (x : Scalar ty0) (y : Scalar ty1)
   (hs : ¬ ty0.isSigned) (hy0 : 0 ≤ y.val) (hy1 : y.val ≤ ty0.bitWidth) :
-  ∃ z, x <<< y = ok z ∧
-  z.val = x.val >>> y.toNat
+  ∃ z, x >>> y = ok z ∧ z.bv_ = x.bv_ >>> y.toNat
   := by
   sorry
+
+@[pspec] theorem U8.ShiftRight_bv_unsigned_eq (x : U8) (y : Scalar ty1) (hy0 : 0 ≤ y.val) (hy1 : y.val ≤ 8) :
+  ∃ (z : U8), x >>> y = ok z ∧ z.bv = x.bv >>> y.toNat
+  := by apply core.num.Scalar.ShiftRight_bv_unsigned_eq <;> simp [*]
+
+@[pspec] theorem U16.ShiftRight_bv_unsigned_eq (x : U16) (y : Scalar ty1) (hy0 : 0 ≤ y.val) (hy1 : y.val ≤ 16) :
+  ∃ (z : U16), x >>> y = ok z ∧ z.bv = x.bv >>> y.toNat
+  := by apply core.num.Scalar.ShiftRight_bv_unsigned_eq <;> simp [*]
+
+@[pspec] theorem U32.ShiftRight_bv_unsigned_eq (x : U32) (y : Scalar ty1) (hy0 : 0 ≤ y.val) (hy1 : y.val ≤ 32) :
+  ∃ (z : U32), x >>> y = ok z ∧ z.bv = x.bv >>> y.toNat
+  := by apply core.num.Scalar.ShiftRight_bv_unsigned_eq <;> simp [*]
+
+@[pspec] theorem U64.ShiftRight_bv_unsigned_eq (x : U64) (y : Scalar ty1) (hy0 : 0 ≤ y.val) (hy1 : y.val ≤ 64) :
+  ∃ (z : U64), x >>> y = ok z ∧ z.bv = x.bv >>> y.toNat
+  := by apply core.num.Scalar.ShiftRight_bv_unsigned_eq <;> simp [*]
+
+@[pspec] theorem U128.ShiftRight_bv_unsigned_eq (x : U128) (y : Scalar ty1) (hy0 : 0 ≤ y.val) (hy1 : y.val ≤ 128) :
+  ∃ (z : U128), x >>> y = ok z ∧ z.bv = x.bv >>> y.toNat
+  := by apply core.num.Scalar.ShiftRight_bv_unsigned_eq <;> simp [*]
+
+@[pspec] theorem Usize.ShiftRight_bv_unsigned_eq (x : Usize) (y : Scalar ty1) (hy0 : 0 ≤ y.val) (hy1 : y.val ≤ size_num_bits) :
+  ∃ (z : Usize), x >>> y = ok z ∧ z.bv = x.bv >>> y.toNat
+  := by apply core.num.Scalar.ShiftRight_bv_unsigned_eq <;> simp_all
+
+theorem core.num.Scalar.ShiftLeft_val_unsigned_eq {ty0 ty1} (x : Scalar ty0) (y : Scalar ty1)
+  (hs : ¬ ty0.isSigned) (hy0 : 0 ≤ y.val) (hy1 : y.val ≤ ty0.bitWidth) :
+  ∃ z, x <<< y = ok z ∧ z.val = x.val <<< y.val -- TODO: can't use y.toNat?
+  := by
+  sorry
+
+theorem core.num.Scalar.ShiftLeft_bv_unsigned_eq {ty0 ty1} (x : Scalar ty0) (y : Scalar ty1)
+  (hs : ¬ ty0.isSigned) (hy0 : 0 ≤ y.val) (hy1 : y.val ≤ ty0.bitWidth) :
+  ∃ z, x <<< y = ok z ∧ z.bv_ = x.bv_ <<< y.toNat
+  := by
+  sorry
+
+@[pspec] theorem U8.ShiftLeft_bv_unsigned_eq (x : U8) (y : Scalar ty1) (hy0 : 0 ≤ y.val) (hy1 : y.val ≤ 8) :
+  ∃ (z : U8), x <<< y = ok z ∧ z.bv = x.bv <<< y.toNat
+  := by apply core.num.Scalar.ShiftLeft_bv_unsigned_eq <;> simp [*]
+
+@[pspec] theorem U16.ShiftLeft_bv_unsigned_eq (x : U16) (y : Scalar ty1) (hy0 : 0 ≤ y.val) (hy1 : y.val ≤ 16) :
+  ∃ (z : U16), x <<< y = ok z ∧ z.bv = x.bv <<< y.toNat
+  := by apply core.num.Scalar.ShiftLeft_bv_unsigned_eq <;> simp [*]
+
+@[pspec] theorem U32.ShiftLeft_bv_unsigned_eq (x : U32) (y : Scalar ty1) (hy0 : 0 ≤ y.val) (hy1 : y.val ≤ 32) :
+  ∃ (z : U32), x <<< y = ok z ∧ z.bv = x.bv <<< y.toNat
+  := by apply core.num.Scalar.ShiftLeft_bv_unsigned_eq <;> simp [*]
+
+@[pspec] theorem U64.ShiftLeft_bv_unsigned_eq (x : U64) (y : Scalar ty1) (hy0 : 0 ≤ y.val) (hy1 : y.val ≤ 64) :
+  ∃ (z : U64), x <<< y = ok z ∧ z.bv = x.bv <<< y.toNat
+  := by apply core.num.Scalar.ShiftLeft_bv_unsigned_eq <;> simp [*]
+
+@[pspec] theorem U128.ShiftLeft_bv_unsigned_eq (x : U128) (y : Scalar ty1) (hy0 : 0 ≤ y.val) (hy1 : y.val ≤ 128) :
+  ∃ (z : U128), x <<< y = ok z ∧ z.bv = x.bv <<< y.toNat
+  := by apply core.num.Scalar.ShiftLeft_bv_unsigned_eq <;> simp [*]
+
+@[pspec] theorem Usize.ShiftLeft_bv_unsigned_eq (x : Usize) (y : Scalar ty1) (hy0 : 0 ≤ y.val) (hy1 : y.val ≤ size_num_bits) :
+  ∃ (z : Usize), x <<< y = ok z ∧ z.bv = x.bv <<< y.toNat
+  := by apply core.num.Scalar.ShiftLeft_bv_unsigned_eq <;> simp_all
 
 end Aeneas.Std
 
@@ -243,7 +352,7 @@ theorem massert_decide_spec (b : Prop) [Decidable b] (h : b) :
 
 -- TODO: generalize, move
 @[simp] theorem core.num.U32.and_val (x y : U32) :
-  (x &&& y).val = Int.land x.val y.val := by
+  (x &&& y).val = (x.bv &&& y.bv).toNat := by
   sorry
 
 -- TODO: move
@@ -324,8 +433,6 @@ theorem Int.testBit_two_pow_sub_succ {x : Int} {n : ℕ} (h₁ : 0 ≤ x) (h₂ 
     sorry
   simp [this]
 
-#check Nat.testBit_shiftRight
-
 @[simp] theorem Int.testBit_shiftRight {i j : Nat} (x : Int) :
   (x >>> i).testBit j = x.testBit (i + j) := by
   sorry
@@ -343,35 +450,158 @@ theorem Int.testBit_pos_eq_false_of_lt {n : Int} {i : ℕ} (h : 0 ≤ n) (h : n 
   n.testBit i = false := by
   sorry
 
--- TODO: move
-theorem ntt.SymCryptMlKemMod_underflow_eq
-  (n m : Int) (hn0 : 0 ≤ n) (hn : n < 2 ^ 12) (hm0 : 0 ≤ m) (hm : m < 2 ^ 12):
-  Int.land m ((2^32 - 1 - n) >>> (16 : Nat)) = m := by
-  apply Int.eq_of_testBit_eq
-  intro i
-  have h : 2^32 - 1 - n = 2^32 - (n + 1) := by ring_nf
-  rw [h]; clear h
-  have := @Int.testBit_two_pow_sub_succ n 32 (by omega) (by omega) (16 + i)
-  simp [-Int.reducePow]
-  rw [this]; clear this
-  intro hi
-  dcases hi : i < 12
-  . simp; split_conjs
-    . omega
-    . have hi : n < 2^(16 + i) := by
-        have := @Int.pow_le_pow_of_le_right 2 (by simp) 12 (16 + i) (by omega)
-        norm_cast at *
-        omega
-      apply @Int.testBit_pos_eq_false_of_lt n (16 + i) (by omega) hi
-  . -- Contradiction
-    have hi : m < 2^i := by
-      have := @Int.pow_le_pow_of_le_right 2 (by simp) 12 i (by omega)
-      norm_cast at *
-      omega
-    have := @Int.testBit_pos_eq_false_of_lt m i (by omega) hi
-    simp_all
-
 #check Aeneas.Std.core.num.Scalar.ShiftRight_val_unsigned_eq
+
+#check Scalar.eq_equiv
+
+theorem Scalar.eq_equiv_bv__eq {ty : ScalarTy} (x y : Scalar ty) :
+  x = y ↔ x.bv_ = y.bv_ := by
+  rw [Scalar.eq_equiv]
+  rw [BitVec.toNat_eq]
+  unfold Scalar.bv_
+  split <;> simp <;>
+  sorry
+
+theorem U8.eq_equiv_bv_eq (x y : U8) : x = y ↔ x.bv = y.bv := by apply Scalar.eq_equiv_bv__eq
+theorem U16.eq_equiv_bv_eq (x y : U16) : x = y ↔ x.bv = y.bv := by apply Scalar.eq_equiv_bv__eq
+theorem U32.eq_equiv_bv_eq (x y : U32) : x = y ↔ x.bv = y.bv := by apply Scalar.eq_equiv_bv__eq
+theorem U64.eq_equiv_bv_eq (x y : U64) : x = y ↔ x.bv = y.bv := by apply Scalar.eq_equiv_bv__eq
+theorem U128.eq_equiv_bv_eq (x y : U128) : x = y ↔ x.bv = y.bv := by apply Scalar.eq_equiv_bv__eq
+theorem Usize.eq_equiv_bv_eq (x y : Usize) : x = y ↔ x.bv = y.bv := by apply Scalar.eq_equiv_bv__eq
+
+theorem Scalar.ofIntCore_bv {ty : ScalarTy} (x : Int) h :
+  (@Scalar.ofIntCore ty x h).bv_ = if ty.isSigned then BitVec.ofInt _ x else BitVec.ofNat _ x.toNat :=
+  by sorry
+
+@[simp] theorem U8.ofInt_bv (x : Int) h : U8.bv (U8.ofInt x h) = BitVec.ofNat _ x.toNat := by apply Scalar.ofIntCore_bv
+@[simp] theorem U16.ofInt_bv (x : Int) h : U16.bv (U16.ofInt x h) = BitVec.ofNat _ x.toNat := by apply Scalar.ofIntCore_bv
+@[simp] theorem U32.ofInt_bv (x : Int) h : U32.bv (U32.ofInt x h) = BitVec.ofNat _ x.toNat := by apply Scalar.ofIntCore_bv
+@[simp] theorem U64.ofInt_bv (x : Int) h : U64.bv (U64.ofInt x h) = BitVec.ofNat _ x.toNat := by apply Scalar.ofIntCore_bv
+@[simp] theorem U128.ofInt_bv (x : Int) h : U128.bv (U128.ofInt x h) = BitVec.ofNat _ x.toNat := by apply Scalar.ofIntCore_bv
+@[simp] theorem Usize.ofInt_bv (x : Int) h : Usize.bv (Usize.ofInt x h) = BitVec.ofNat _ x.toNat := by apply Scalar.ofIntCore_bv
+
+theorem Scalar.add_bv_spec {ty} {x y : Scalar ty} (hmin : Scalar.min ty ≤ x.val + y.val) (hmax : x.val + y.val ≤ Scalar.max ty) :
+  ∃ (z : Scalar ty), x + y = ok z ∧ z.val = x.val + y.val ∧ z.bv_ = x.bv_ + y.bv_ := by sorry
+
+theorem U8.add_bv_spec {x y : U8} (hmax : x.val + y.val ≤ U8.max) :
+  ∃ (z : U8), x + y = ok z ∧ z.val = x.val + y.val ∧ z.bv = x.bv + y.bv :=
+  by apply Scalar.add_bv_spec; scalar_tac; apply hmax
+
+theorem U16.add_bv_spec {x y : U16} (hmax : x.val + y.val ≤ U16.max) :
+  ∃ (z : U16), x + y = ok z ∧ z.val = x.val + y.val ∧ z.bv = x.bv + y.bv :=
+  by apply Scalar.add_bv_spec; scalar_tac; apply hmax
+
+theorem U32.add_bv_spec {x y : U32} (hmax : x.val + y.val ≤ U32.max) :
+  ∃ (z : U32), x + y = ok z ∧ z.val = x.val + y.val ∧ z.bv = x.bv + y.bv :=
+  by apply Scalar.add_bv_spec; scalar_tac; apply hmax
+
+theorem U64.add_bv_spec {x y : U64} (hmax : x.val + y.val ≤ U64.max) :
+  ∃ (z : U64), x + y = ok z ∧ z.val = x.val + y.val ∧ z.bv = x.bv + y.bv :=
+  by apply Scalar.add_bv_spec; scalar_tac; apply hmax
+
+theorem U128.add_bv_spec {x y : U128} (hmax : x.val + y.val ≤ U128.max) :
+  ∃ (z : U128), x + y = ok z ∧ z.val = x.val + y.val ∧ z.bv = x.bv + y.bv :=
+  by apply Scalar.add_bv_spec; scalar_tac; apply hmax
+
+theorem Usize.add_bv_spec {x y : Usize} (hmax : x.val + y.val ≤ Usize.max) :
+  ∃ (z : Usize), x + y = ok z ∧ z.val = x.val + y.val ∧ z.bv = x.bv + y.bv :=
+  by apply Scalar.add_bv_spec; scalar_tac; apply hmax
+
+theorem I8.add_bv_spec {x y : I8} (hmin : I8.min ≤ x.val + y.val) (hmax : x.val + y.val ≤ I8.max) :
+  ∃ (z : I8), x + y = ok z ∧ z.val = x.val + y.val ∧ z.bv = x.bv + y.bv :=
+  by apply Scalar.add_bv_spec <;> scalar_tac
+
+theorem I16.add_bv_spec {x y : I16} (hmin : I16.min ≤ x.val + y.val) (hmax : x.val + y.val ≤ I16.max) :
+  ∃ (z : I16), x + y = ok z ∧ z.val = x.val + y.val ∧ z.bv = x.bv + y.bv :=
+  by apply Scalar.add_bv_spec <;> scalar_tac
+
+theorem I32.add_bv_spec {x y : I32} (hmin : I32.min ≤ x.val + y.val) (hmax : x.val + y.val ≤ I32.max) :
+  ∃ (z : I32), x + y = ok z ∧ z.val = x.val + y.val ∧ z.bv = x.bv + y.bv :=
+  by apply Scalar.add_bv_spec <;> scalar_tac
+
+theorem I64.add_bv_spec {x y : I64} (hmin : I64.min ≤ x.val + y.val) (hmax : x.val + y.val ≤ I64.max) :
+  ∃ (z : I64), x + y = ok z ∧ z.val = x.val + y.val ∧ z.bv = x.bv + y.bv :=
+  by apply Scalar.add_bv_spec <;> scalar_tac
+
+theorem I128.add_bv_spec {x y : I128} (hmin : I128.min ≤ x.val + y.val) (hmax : x.val + y.val ≤ I128.max) :
+  ∃ (z : I128), x + y = ok z ∧ z.val = x.val + y.val ∧ z.bv = x.bv + y.bv :=
+  by apply Scalar.add_bv_spec <;> scalar_tac
+
+theorem Isize.add_bv_spec {x y : Isize} (hmin : Isize.min ≤ x.val + y.val) (hmax : x.val + y.val ≤ Isize.max) :
+  ∃ (z : Isize), x + y = ok z ∧ z.val = x.val + y.val ∧ z.bv = x.bv + y.bv :=
+  by apply Scalar.add_bv_spec <;> scalar_tac
+
+theorem Scalar.unsigned_ofInt_bv_lt_equiv {ty} (h : ¬ ty.isSigned) (x y : Int) (hx) (hy) :
+  (@Scalar.ofInt ty x hx).bv_ < (@Scalar.ofInt ty y hy).bv_ ↔ x < y := by
+  sorry
+
+@[simp] theorem U8.toNat_mod_max_eq (x : U8) : x.toNat % (U8.max + 1) = x.toNat := by
+  apply Nat.mod_eq_of_lt; scalar_tac
+
+@[simp] theorem U8.toNat_mod_max_eq' (x : U8) : x.toNat % 256 = x.toNat := by
+  apply Nat.mod_eq_of_lt; scalar_tac
+
+@[simp] theorem U16.toNat_mod_max_eq (x : U16) : x.toNat % (U16.max + 1) = x.toNat := by
+  apply Nat.mod_eq_of_lt; scalar_tac
+
+@[simp] theorem U16.toNat_mod_max_eq' (x : U16) : x.toNat % 65536 = x.toNat := by
+  apply Nat.mod_eq_of_lt; scalar_tac
+
+@[simp] theorem U32.toNat_mod_max_eq (x : U32) : x.toNat % (U32.max + 1) = x.toNat := by
+  apply Nat.mod_eq_of_lt; scalar_tac
+
+@[simp] theorem U32.toNat_mod_max_eq' (x : U32) : x.toNat % 4294967296 = x.toNat := by
+  apply Nat.mod_eq_of_lt; scalar_tac
+
+@[simp] theorem U64.toNat_mod_max_eq (x : U64) : x.toNat % (U64.max + 1) = x.toNat := by
+  apply Nat.mod_eq_of_lt; scalar_tac
+
+@[simp] theorem U64.toNat_mod_max_eq' (x : U64) : x.toNat % 18446744073709551616 = x.toNat := by
+  apply Nat.mod_eq_of_lt; scalar_tac
+
+@[simp] theorem U128.toNat_mod_max_eq (x : U128) : x.toNat % (U128.max + 1) = x.toNat := by
+  apply Nat.mod_eq_of_lt; scalar_tac
+
+@[simp] theorem U128.toNat_mod_max_eq' (x : U128) : x.toNat % 340282366920938463463374607431768211456 = x.toNat := by
+  apply Nat.mod_eq_of_lt; scalar_tac
+
+@[simp] theorem Usize.toNat_mod_max_eq (x : Usize) : x.toNat % (Usize.max + 1) = x.toNat := by
+  apply Nat.mod_eq_of_lt; scalar_tac
+
+@[simp] theorem U8.val_mod_max_eq (x : U8) : x.val % (U8.max + 1) = x.val := by
+  apply Int.emod_eq_of_lt <;> scalar_tac
+
+@[simp] theorem U8.val_mod_max_eq' (x : U8) : x.val % 256 = x.val := by
+  apply Int.emod_eq_of_lt <;> scalar_tac
+
+@[simp] theorem U16.val_mod_max_eq (x : U16) : x.val % (U16.max + 1) = x.val := by
+  apply Int.emod_eq_of_lt <;> scalar_tac
+
+@[simp] theorem U16.val_mod_max_eq' (x : U16) : x.val % 65536 = x.val := by
+  apply Int.emod_eq_of_lt <;> scalar_tac
+
+@[simp] theorem U32.val_mod_max_eq (x : U32) : x.val % (U32.max + 1) = x.val := by
+  apply Int.emod_eq_of_lt <;> scalar_tac
+
+@[simp] theorem U32.val_mod_max_eq' (x : U32) : x.val % 4294967296 = x.val := by
+  apply Int.emod_eq_of_lt <;> scalar_tac
+
+@[simp] theorem U64.val_mod_max_eq (x : U64) : x.val % (U64.max + 1) = x.val := by
+  apply Int.emod_eq_of_lt <;> scalar_tac
+
+@[simp] theorem U64.val_mod_max_eq' (x : U64) : x.val % 18446744073709551616 = x.val := by
+  apply Int.emod_eq_of_lt <;> scalar_tac
+
+@[simp] theorem U128.val_mod_max_eq (x : U128) : x.val % (U128.max + 1) = x.val := by
+  apply Int.emod_eq_of_lt <;> scalar_tac
+
+@[simp] theorem U128.val_mod_max_eq' (x : U128) : x.val % 340282366920938463463374607431768211456 = x.val := by
+  apply Int.emod_eq_of_lt <;> scalar_tac
+
+@[simp] theorem Usize.val_mod_max_eq (x : Usize) : x.val % (Usize.max + 1) = x.val := by
+  apply Int.emod_eq_of_lt <;> scalar_tac
+
+-- TODO: improve scalar_tac to reason about inequalities between bitvectors?
 
 theorem ntt.SymCryptMlKemMod'_spec (a : U32) (b : U32)
   (ha : a.val < Spec.Q) (hb : b.val < Spec.Q) :
@@ -379,34 +609,55 @@ theorem ntt.SymCryptMlKemMod'_spec (a : U32) (b : U32)
   (c.val : Spec.Zq) = (a.val : Spec.Zq) + (b.val : Spec.Zq) ∧
   c.val < Spec.Q := by
   unfold SymCryptMlKemModAdd'
+  -- TODO: automate those
+  have : a.bv < 3329#32 := by
+    simp [U32.bv, Scalar.bv_]
+    scalar_tac
+  have : b.bv < 3329#32 := by
+    simp [U32.bv, Scalar.bv_]
+    scalar_tac
   simp at *
   progress
   progress
-  progress as ⟨ c1, hc1 ⟩
+  progress with U32.add_bv_spec as ⟨ c1, hc1 ⟩
   progress as ⟨ c2, hc2 ⟩
   simp at *
+
   -- TODO: handle this properly with progress
   have hIf : (if c2 = 0#u32 then ok () else massert (c2 = 65535#u32)) = ok () := by
-    split <;> simp_all
-    sorry
+    split <;> try simp
+    progress
+    simp [U32.eq_equiv_bv_eq] at *
+    bv_decide
   progress; clear hIf
-  --
-  progress
-  . sorry -- This is the assert
-  . simp
+
+  -- Prove the post-condition
+  have hPost :
+    let c := core.num.U32.wrapping_add (core.num.U32.wrapping_sub c1 3329#u32) (3329#u32 &&& c2)
+    (c.val : Spec.Zq) = (a.val : Spec.Zq) + (b.val : Spec.Zq) ∧
+    c.val < Spec.Q := by
+    simp
     -- There are two cases depending on whether `a + b - q` is `< 0` or not
     dcases hlt : 0 ≤ a.val + b.val - 3329
     . -- No underflow
+      -- TODO: automate
+      have : 3329#32 ≤ a.bv + b.bv := by
+        simp [BitVec.le_def]
+        rw [Nat.mod_eq_of_lt] <;> omega
+
+      -- The important part of the proof, that we prove with bv_decide
+      have hc2Eq : c2.toNat = 0 := by -- TODO: automate
+        have h : c2.bv = 0#32 := by bv_decide
+        have h : c2.bv.toNat = 0 := by rw [h]; simp
+        simp at h
+        scalar_tac
+      simp [hc2Eq]; clear hc2
+
       let c : Int := a.val + b.val - 3329
       have : 0 ≤ c ∧ c < 3329 := by scalar_tac
       have hcMod : c % (U32.max + 1) = c := by
         apply Int.emod_eq_of_lt <;> scalar_tac
-      have hc2Eq : c2.val = 0 := by
-        rw [hc2, hc1, hcMod]
-        rw [Int.shiftRight_eq_div_pow]
-        apply Int.ediv_eq_zero_of_lt <;>
-        scalar_tac
-      rw [hc2Eq]
+
       simp [*]
       rw [hcMod]
       simp +zetaDelta [Spec.Zq]
@@ -415,32 +666,30 @@ theorem ntt.SymCryptMlKemMod'_spec (a : U32) (b : U32)
       . scalar_tac
     . -- Underflow
       simp at hlt
-      have hAnd : Int.land 3329 c2.val = 3329 := by
-        -- This is the tricky proof
-        have hc1Mod :=
-          calc
-            (c1.val - 3329) % (U32.max + 1) =
-              (U32.max + 1 - (3329 - c1.val)) % (U32.max + 1) := by
-              have := @Int.add_emod_self_left (U32.max + 1) (c1.val - 3329)
-              rw [← this]
-              ring_nf
-            _ = U32.max + 1 - (3329 - c1.val) := by
-              apply Int.emod_eq_of_lt <;> scalar_tac
 
-        rw [hc2, hc1Mod]
-        have hEq := ntt.SymCryptMlKemMod_underflow_eq (3329 - c1.val - 1) 3329 (by scalar_tac) (by scalar_tac) (by simp) (by simp)
-        ring_nf at hEq
-        simp [U32.max]
-        ring_nf
-        apply hEq
-      rw [hAnd]
-      simp
+      have : a.bv + b.bv < 3329#32 := by
+        simp [BitVec.lt_def]
+        rw [Nat.mod_eq_of_lt] <;> omega
 
-      have hMod : c1.val % (U32.max + 1) = c1.val := by
-        apply Int.emod_eq_of_lt <;> scalar_tac
-      rw [hMod]
+      -- The important part of the proof, that we prove with bv_decide
+      have hc2Eq : 3329 &&& c2.toNat = 3329 := by -- TODO: automate
+        have h : 3329#32 &&& c2.bv = 3329#32 := by bv_decide
+        have h : (3329#32 &&& c2.bv).toNat = 3329 := by
+          simp [h]
+        simp at h
+        apply h
+      simp [hc2Eq]; clear hc2
+
       split_conjs
       . simp [*]
       . scalar_tac
+
+  -- Finish the proof
+  progress
+  . -- massert
+    simp at hPost
+    apply hPost.right
+  . simp at *
+    apply hPost
 
 end Symcrust
